LogicalRefinement/Stlc/Subst.lean
@@ -4,11 +4,11 @@ import LogicalRefinement.Stlc.Basic
 import LogicalRefinement.Stlc.Interp
 
 def Stlc.InterpSubst (Γ Δ: Context): Type := 
-  ∀{n A}, Stlc.HasVar Δ n A -> Γ.deriv A
+  ∀n A, Stlc.HasVar Δ n A -> Γ.deriv A
 
 def Stlc.InterpSubst.pop {H Γ Δ} (S: InterpSubst Γ (H::Δ))
   : InterpSubst Γ Δ
-  := λHv => S Hv.succ
+  := λn A Hv => S _ _ Hv.succ
 
 def Stlc.InterpSubst.lift {H Γ Δ} (S: InterpSubst Γ Δ)
   : InterpSubst (H::Γ) (H::Δ)
@@ -21,7 +21,7 @@ def Stlc.InterpSubst.lift {H Γ Δ} (S: InterpSubst Γ Δ)
       exact HasVar.zero.interp G
     | succ n =>
       let (x, G) := G;
-      exact S (by cases Hv; assumption) G
+      exact S _ _ (by cases Hv; assumption) G
   }
 
 def Stlc.InterpSubst.lift2 {A B Γ Δ} (S: InterpSubst Γ Δ)
@@ -30,7 +30,7 @@ def Stlc.InterpSubst.lift2 {A B Γ Δ} (S: InterpSubst Γ Δ)
 
 def Stlc.InterpSubst.step {H Γ Δ} (S: InterpSubst Γ Δ)
   : InterpSubst (H::Γ) Δ
-  := λHv => (S Hv).step H
+  := λn A Hv => (S _ _ Hv).step H
 
 def Stlc.InterpSubst.pop_lift_step {H Γ Δ} (S: InterpSubst Γ Δ)
   : @pop H (H::Γ) Δ (@lift H Γ Δ S) = @step H Γ Δ S
@@ -50,7 +50,7 @@ def Stlc.InterpSubst.pop_step_commute {A B Γ Δ} (S: InterpSubst Γ (A::Δ))
 
 def Stlc.SubstCtx.interp {σ Γ Δ} (S: SubstCtx σ Γ Δ)
   : Stlc.InterpSubst Γ Δ
-  := λHv => (S Hv).interp
+  := λn A Hv => (S Hv).interp
   
 def Stlc.SubstCtx.pop_interp {σ Γ Δ H} (S: SubstCtx σ Γ (H::Δ))
   : @Stlc.InterpSubst.pop H Γ Δ S.interp
@@ -95,7 +95,7 @@ def Stlc.InterpSubst.transport_ctx {Γ Δ: Context} (S: InterpSubst Γ Δ)
   : Δ.interp
   := match Δ with
      | [] => ()
-     | A::Δ => (S HasVar.zero G, transport_ctx S.pop G)
+     | A::Δ => (S 0 _ HasVar.zero G, transport_ctx S.pop G)
 
 
 def second_helper {a a': A} {f: A -> B}: a = a' -> f a = f a' := by intros; simp [*]
@@ -103,7 +103,7 @@ def pair_helper: a = a' -> b = b' -> (a, b) = (a', b') := by intros; simp [*]
 theorem Stlc.InterpSubst.transport_helper {Γ Δ: Context} {H: Ty} 
   (S: InterpSubst Γ (H::Δ))
   (G: Γ.interp)
-  : S.transport_ctx G = (S HasVar.zero G, transport_ctx S.pop G)
+  : S.transport_ctx G = (S 0 _ HasVar.zero G, transport_ctx S.pop G)
   := by rfl
 
 def Stlc.InterpSubst.transport_step {Γ Δ: Context} {H: Ty} (S: InterpSubst Γ Δ)
